library/init/meta/converter/conv.lean
@@ -6,282 +6,112 @@ Authors: Leonardo de Moura
 Converter monad for building simplifiers.
 -/
 prelude
-import init.meta.tactic init.meta.simp_tactic
+import init.meta.tactic init.meta.simp_tactic init.meta.interactive
 import init.meta.congr_lemma init.meta.match_tactic
 open tactic
 
-meta structure conv_result (α : Type) :=
-(val : α) (rhs : expr) (proof : option expr)
+universe u
 
-meta def conv (α : Type) : Type :=
-name → expr → tactic (conv_result α)
-
-namespace conv
-
-meta def lhs : conv expr :=
-λ r e, return ⟨e, e, none⟩
-
-meta def change (new_p : pexpr) : conv unit :=
-λ r e, do
-  e_type ← infer_type e,
-  new_e ← to_expr ``(%%new_p : %%e_type),
-  unify e new_e,
-  return ⟨(), new_e, none⟩
-
-protected meta def pure {α : Type} : α → conv α :=
-λ a r e, return ⟨a, e, none⟩
-
-private meta def join_proofs (r : name) (o₁ o₂ : option expr) : tactic (option expr) :=
-match o₁, o₂ with
-| none,    _       := return o₂
-| _,       none    := return o₁
-| some p₁, some p₂ := do
-  env ← get_env,
-  match env.trans_for r with
-  | some trans := do pr ← mk_app trans [p₁, p₂], return $ some pr
-  | none       := fail format!"converter failed, relation '{r}' is not transitive"
-  end
-end
-
-protected meta def seq {α β : Type} (c₁ : conv (α → β)) (c₂ : conv α) : conv β :=
-λ r e, do
-  ⟨fn, e₁, pr₁⟩ ← c₁ r e,
-  ⟨a,  e₂, pr₂⟩ ← c₂ r e₁,
-  pr            ← join_proofs r pr₁ pr₂,
-  return ⟨fn a, e₂, pr⟩
-
-protected meta def fail {α β : Type} [has_to_format β] (msg : β) : conv α :=
-λ r e, tactic.fail msg
-
-protected meta def failed {α : Type} : conv α :=
-λ r e, tactic.failed
-
-protected meta def orelse {α : Type} (c₁ : conv α) (c₂ : conv α) : conv α :=
-λ r e, c₁ r e <|> c₂ r e
-
-protected meta def map {α β : Type} (f : α → β) (c : conv α) : conv β :=
-λ r e, do
-  ⟨a, e₁, pr⟩ ← c r e,
-  return ⟨f a, e₁, pr⟩
-
-protected meta def bind {α β : Type} (c₁ : conv α) (c₂ : α → conv β) : conv β :=
-λ r e, do
-  ⟨a, e₁, pr₁⟩ ← c₁ r e,
-  ⟨b, e₂, pr₂⟩ ← c₂ a r e₁,
-  pr           ← join_proofs r pr₁ pr₂,
-  return ⟨b, e₂, pr⟩
+meta def conv (α : Type u) :=
+tactic α
 
 meta instance : monad conv :=
-{ map  := @conv.map,
-  pure := @conv.pure,
-  bind := @conv.bind,
-  id_map := undefined, pure_bind := undefined, bind_assoc := undefined,
-  bind_pure_comp_eq_map := undefined, bind_map_eq_seq := undefined }
+by unfold conv; apply_instance
+
+meta instance : monad_fail conv :=
+by unfold conv; apply_instance
 
 meta instance : alternative conv :=
-{ conv.monad with
-  failure := @conv.failed,
-  orelse  := @conv.orelse }
+by unfold conv; apply_instance
 
-meta def whnf (md : transparency := reducible) : conv unit :=
-λ r e, do n ← tactic.whnf e md, return ⟨(), n, none⟩
+namespace conv
+meta def convert (c : conv unit) (lhs : expr) (rel : name := `eq) : tactic (expr × expr) :=
+do lhs_type   ← infer_type lhs,
+   rhs        ← mk_meta_var lhs_type,
+   new_target ← mk_app rel [lhs, rhs],
+   new_g      ← mk_meta_var new_target,
+   gs         ← get_goals,
+   set_goals [new_g],
+   c,
+   repeat reflexivity,
+   n          ← num_goals,
+   when (n ≠ 0) (fail "convert tactic failed, there are unsolved goals"),
+   set_goals gs,
+   rhs        ← instantiate_mvars rhs,
+   new_g      ← instantiate_mvars new_g,
+   return (rhs, new_g)
 
-meta def dsimp : conv unit :=
-λ r e, do s ← simp_lemmas.mk_default, n ← s.dsimplify e, return ⟨(), n, none⟩
+meta def lhs : conv expr :=
+do (_, lhs, rhs) ← target_lhs_rhs,
+   return lhs
 
-meta def try (c : conv unit) : conv unit :=
-c <|> return ()
+meta def rhs : conv expr :=
+do (_, lhs, rhs) ← target_lhs_rhs,
+   return rhs
 
-meta def tryb (c : conv unit) : conv bool :=
-(c >> return tt) <|> return ff
+meta def update_lhs (new_lhs : expr) (h : expr) : conv unit :=
+do transitivity,
+   rhs >>= unify new_lhs,
+   exact h,
+   t ← target >>= instantiate_mvars,
+   change t
 
-meta def trace {α : Type} [has_to_tactic_format α] (a : α) : conv unit :=
-λ r e, tactic.trace a >> return ⟨(), e, none⟩
-
-meta def trace_lhs : conv unit :=
-lhs >>= trace
-
-meta def apply_lemmas_core (s : simp_lemmas) (prove : tactic unit) : conv unit :=
-λ r e, do
-  (new_e, pr) ← s.rewrite prove r e,
-  return ⟨(), new_e, some pr⟩
-
-meta def apply_lemmas (s : simp_lemmas) : conv unit :=
-apply_lemmas_core s failed
-
-/- adapter for using iff-lemmas as eq-lemmas -/
-meta def apply_propext_lemmas_core (s : simp_lemmas) (prove : tactic unit) : conv unit :=
-λ r e, do
-  guard (r = `eq),
-  (new_e, pr) ← s.rewrite prove `iff e,
-  new_pr ← mk_app `propext [pr],
-  return ⟨(), new_e, some new_pr⟩
-
-meta def apply_propext_lemmas (s : simp_lemmas) : conv unit :=
-apply_propext_lemmas_core s failed
-
-private meta def mk_refl_proof (r : name) (e : expr) : tactic expr :=
-do env ← get_env,
-   match (environment.refl_for env r) with
-   | (some refl) := do pr ← mk_app refl [e], return pr
-   | none        := fail format!"converter failed, relation '{r}' is not reflexive"
-   end
-
-meta def to_tactic (c : conv unit) : name → expr → tactic (expr × expr) :=
-λ r e, do
-  ⟨u, e₁, o⟩ ← c r e,
-  match o with
-  | none   := do p ← mk_refl_proof r e, return (e₁, p)
-  | some p := return (e₁, p)
-  end
-
-meta def lift_tactic {α : Type} (t : tactic α) : conv α :=
-λ r e, do a ← t, return ⟨a, e, none⟩
-
-meta def apply_simp_set (attr_name : name) : conv unit :=
-lift_tactic (get_user_simp_lemmas attr_name) >>= apply_lemmas
-
-meta def apply_propext_simp_set (attr_name : name) : conv unit :=
-lift_tactic (get_user_simp_lemmas attr_name) >>= apply_propext_lemmas
+meta def change (new_lhs : expr) : conv unit :=
+do (r, lhs, rhs) ← target_lhs_rhs,
+   new_target ← mk_app r [new_lhs, rhs],
+   tactic.change new_target
 
 meta def skip : conv unit :=
-return ()
+reflexivity
 
-meta def repeat : conv unit → conv unit
-| c r lhs :=
-  (do
-     ⟨_, rhs₁, pr₁⟩ ← c r lhs,
-     guard (¬ lhs =ₐ rhs₁),
-     ⟨_, rhs₂, pr₂⟩ ← repeat c r rhs₁,
-     pr ← join_proofs r pr₁ pr₂,
-     return ⟨(), rhs₂, pr⟩)
-  <|> return ⟨(), lhs, none⟩
+meta def whnf : conv unit :=
+lhs >>= tactic.whnf >>= change
 
-meta def first {α : Type} : list (conv α) → conv α
-| []      := conv.failed
-| (c::cs) := c <|> first cs
+meta def dsimp (s : option simp_lemmas := none) : conv unit :=
+do s ← match s with
+       | some s := return s
+       | none   := simp_lemmas.mk_default
+       end,
+   lhs >>= s.dsimplify >>= change
 
-meta def match_pattern (p : pattern) : conv unit :=
-λ r e, tactic.match_pattern p e >> return ⟨(), e, none⟩
-
-meta def mk_match_expr (p : pexpr) : tactic (conv unit) :=
-do new_p ← pexpr_to_pattern p,
-   return (λ r e, tactic.match_pattern new_p e >> return ⟨(), e, none⟩)
-
-meta def match_expr (p : pexpr) : conv unit :=
-λ r e, do
-  new_p ← pexpr_to_pattern p,
-  tactic.match_pattern new_p e >> return ⟨(), e, none⟩
-
-meta def funext (c : conv unit) : conv unit :=
-λ r lhs, do
-  guard (r = `eq),
-  (expr.lam n bi d b) ← return lhs,
-  let aux_type := expr.pi n bi d (expr.const `true []),
-  (result, _) ← solve_aux aux_type $ do {
-    x ← intro1,
-    c_result ← c r (b.instantiate_var x),
-    let rhs  := expr.lam n bi d (c_result.rhs.abstract x),
-    match c_result.proof : _ → tactic (conv_result unit) with
-    | some pr := do
-      let aux_pr := expr.lam n bi d (pr.abstract x),
-      new_pr ← mk_app `funext [lhs, rhs, aux_pr],
-      return ⟨(), rhs, some new_pr⟩
-    | none    := return ⟨(), rhs, none⟩
-    end },
-  return result
-
-meta def congr_core (c_f c_a : conv unit) : conv unit :=
-λ r lhs, do
-  guard (r = `eq),
-  (expr.app f a) ← return lhs,
-  f_type ← infer_type f >>= tactic.whnf,
-  guard (f_type.is_arrow),
-  ⟨(), new_f, of⟩ ← try c_f r f,
-  ⟨(), new_a, oa⟩ ← try c_a r a,
-  rhs ← return $ new_f new_a,
-  match of, oa with
-  | none, none      :=
-      return ⟨(), rhs, none⟩
-  | none, some pr_a := do
-      pr ← mk_app `congr_arg [a, new_a, f, pr_a],
-      return ⟨(), new_f new_a, some pr⟩
-  | some pr_f, none := do
-      pr ← mk_app `congr_fun [f, new_f, pr_f, a],
-      return ⟨(), rhs, some pr⟩
-  | some pr_f, some pr_a := do
-      pr ← mk_app `congr [f, new_f, a, new_a, pr_f, pr_a],
-      return ⟨(), rhs, some pr⟩
+private meta def congr_aux : list congr_arg_kind → list expr → tactic (list expr × list expr)
+| []      []      := return ([], [])
+| (k::ks) (a::as) := do
+  (gs, largs) ← congr_aux ks as,
+  match k with
+  | congr_arg_kind.fixed            := return $ (gs, a::largs)
+  | congr_arg_kind.fixed_no_param   := return $ (gs, largs)
+  | congr_arg_kind.eq               := do
+      a_type  ← infer_type a,
+      rhs     ← mk_meta_var a_type,
+      g_type  ← mk_app `eq [a, rhs],
+      g       ← mk_meta_var g_type,
+      return (g::gs, a::rhs::g::largs)
+  | congr_arg_kind.cast             := return $ (gs, a::largs)
+  | _                               := fail "congr tactic failed, unsupported congruence lemma"
   end
+| ks      as := fail "congr tactic failed, unsupported congruence lemma"
 
-meta def congr (c : conv unit) : conv unit :=
-congr_core c c
+meta def congr : conv unit :=
+do (r, lhs, rhs) ← target_lhs_rhs,
+   guard (r = `eq),
+   let fn   := lhs.get_app_fn,
+   let args := lhs.get_app_args,
+   cgr_lemma ← mk_congr_lemma_simp fn (some args.length),
+   g::gs ← get_goals,
+   (new_gs, lemma_args) ← congr_aux cgr_lemma.arg_kinds args,
+   let g_val := cgr_lemma.proof.mk_app lemma_args,
+   unify g g_val,
+   set_goals $ new_gs ++ gs,
+   return ()
 
-meta def bottom_up (c : conv unit) : conv unit :=
-λ r e, do
-  s ← simp_lemmas.mk_default,
-  (a, new_e, pr) ←
-     ext_simplify_core () {} s
-       (λ u, return u)
-       (λ a s r p e, failed)
-       (λ a s r p e, do ⟨u, new_e, pr⟩ ← c r e, return ((), new_e, pr, tt))
-       r e,
-  return ⟨(), new_e, some pr⟩
-
-meta def top_down (c : conv unit) : conv unit :=
-λ r e, do
-  s ← simp_lemmas.mk_default,
-  (a, new_e, pr) ←
-     ext_simplify_core () {} s
-       (λ u, return u)
-       (λ a s r p e, do ⟨u, new_e, pr⟩ ← c r e, return ((), new_e, pr, tt))
-       (λ a s r p e, failed)
-       r e,
-  return ⟨(), new_e, some pr⟩
-
-meta def find (c : conv unit) : conv unit :=
-λ r e, do
-  s ← simp_lemmas.mk_default,
-  (a, new_e, pr) ←
-     ext_simplify_core () {} s
-       (λ u, return u)
-       (λ a s r p e,
-         (do ⟨u, new_e, pr⟩ ← c r e, return ((), new_e, pr, ff))
-         <|>
-         return ((), e, none, tt))
-       (λ a s r p e, failed)
-       r e,
-  return ⟨(), new_e, some pr⟩
-
-meta def find_pattern (pat : pattern) (c : conv unit) : conv unit :=
-λ r e, do
-  s ← simp_lemmas.mk_default,
-  (a, new_e, pr) ←
-     ext_simplify_core () {} s
-       (λ u, return u)
-       (λ a s r p e, do
-         matched ← (tactic.match_pattern pat e >> return tt) <|> return ff,
-         if matched
-         then do ⟨u, new_e, pr⟩ ← c r e, return ((), new_e, pr, ff)
-         else return ((), e, none, tt))
-       (λ a s r p e, failed)
-       r e,
-  return ⟨(), new_e, some pr⟩
-
-meta def findp : pexpr → conv unit → conv unit :=
-λ p c r e, do
-  pat ← pexpr_to_pattern p,
-  find_pattern pat c r e
-
-meta def conversion (c : conv unit) : tactic unit :=
-do (r, lhs, rhs) ← (target_lhs_rhs <|> fail "conversion failed, target is not of the form 'lhs R rhs'"),
-   (new_lhs, pr) ← to_tactic c r lhs,
-   (unify new_lhs rhs <|>
-     do new_lhs_fmt ← pp new_lhs,
-        rhs_fmt     ← pp rhs,
-        fail (to_fmt "conversion failed, expected" ++
-                     rhs_fmt.indent 4 ++ format.line ++ "provided" ++
-                     new_lhs_fmt.indent 4)),
-   exact pr
+meta def funext : conv unit :=
+repeat $ do
+  (r, lhs, rhs) ← target_lhs_rhs,
+  guard (r = `eq),
+  (expr.lam n _ _ _) ← return lhs,
+  tactic.applyc `funext,
+  intro n,
+  return ()
 
 end conv
