tests/lean/run/conv_tac1.lean
@@ -1,6 +1,6 @@
 example (a b : nat) : (λ x, a + x) 0 = b + 1 + a :=
 begin
-  find (_ + 1) { change nat.succ b },
+  conv in (_ + 1) { change nat.succ b },
   guard_target (λ x, a + x) 0 = nat.succ b + a,
   admit
 end
